# estadistica-pucp

## mostreo:

$$\sigma_{xy} = \frac{1}{N-1}\left(S - N\mu_x\mu_y\right)\\
\mathrm{E}\left[\bar X\bar Y\right] = \frac{n}{N}S + \frac{n(n-1)}{N(N-1)}\left(N^2\mu_x\mu_y - S\right)\\
$$
$$\frac{1-N}{n(n-1)}\mathrm{E}\left[\bar X\bar Y\right] = \frac{1-N}{N(n-1)}S - N\mu_x\mu_y + \frac{S}{N}$$

$$\frac{1-N}{n(n-1)}\mathrm{E}\left[\bar{X}\bar{Y}\right] = \frac{n-N}{N(n-1)}S - N\mu_x\mu_y$$

$$s_{xy}=\frac{N-1}{n-1}XY-\frac{N-1}{n(n-1)}\bar{X}\bar{Y}$$

$$s_{xy}=\frac{N-1}{n-1}\left(XY-\bar{X}\bar{Y}\right)$$
